interval_tree.dfy
@@ -1,0 +1,327 @@
+function method min(a: int, b: int) : int
+{
+	if a < b
+		then a
+	else
+		b
+}
+
+function method max(a: int, b: int) : int
+{
+	if a < b
+		then b
+	else
+		a
+}
+
+datatype Endpoint = Open(point: int) | Closed(point: int)
+
+datatype Interval = Interval(low: Endpoint, high: Endpoint)
+	
+predicate method IntervalIsEmpty(ival: Interval) {
+	ival.low.point > ival.high.point ||
+		(ival.low.point == ival.high.point && (ival.low.Open? || ival.high.Open?))
+}
+
+predicate method IntervalContains(ival: Interval, value: int)
+{
+	(if ival.low.Closed? then ival.low.point <= value else ival.low.point < value)	&&
+		(if ival.high.Closed? then value <= ival.high.point else value < ival.high.point)
+}
+
+predicate method IsSubInterval(ival1: Interval, ival2: Interval)
+	ensures IsSubInterval(ival1, ival2) ==> forall x: int :: IntervalContains(ival1, x) ==> IntervalContains(ival2, x);
+{
+	IntervalIsEmpty(ival1) ||
+		((ival2.low.point <= ival1.low.point) &&
+		(ival2.low.point == ival1.low.point ==> ival2.low.Closed? || ival1.low.Open?) &&
+		(ival2.high.point >= ival1.high.point) &&
+		(ival2.high.point == ival1.high.point ==> ival2.high.Closed? || ival1.high.Open?))
+}
+
+function method IntervalUnion(a: Interval, b: Interval) : Interval
+	ensures IsSubInterval(a, IntervalUnion(a, b));
+	ensures IsSubInterval(b, IntervalUnion(a, b));
+{
+	if IntervalIsEmpty(a) && IntervalIsEmpty(b) then
+		Interval(Open(0), Open(0))
+	else if IntervalIsEmpty(a) then
+		b
+	else if IntervalIsEmpty(b) then
+		a
+	else
+		var low := min(a.low.point, b.low.point);
+		var lowep := if a.low.Closed? || b.low.Closed? then Closed(low) else Open(low);
+		var high := max(a.high.point, b.high.point);
+		var highep := if a.high.Closed? || b.high.Closed? then Closed(high) else Open(high);
+		Interval(lowep, highep)
+}
+
+function method IntervalUnion3(a: Interval, b: Interval, c: Interval) : Interval
+	ensures IsSubInterval(a, IntervalUnion3(a, b, c));
+	ensures IsSubInterval(b, IntervalUnion3(a, b,c ));
+	ensures IsSubInterval(c, IntervalUnion3(a, b,c ));
+{
+	IntervalUnion(a, IntervalUnion(b, c))
+}
+
+datatype Node =
+	Leaf(value: Interval) |
+	TwoNode(left: Node, pivot: int, right: Node, interval: Interval) |
+	ThreeNode(left: Node, pivota: int, middle: Node, pivotb: int, right: Node, interval: Interval)
+
+function method SummaryInterval(tree: Node) : Interval {
+	if tree.Leaf? then tree.value else tree.interval
+}
+	
+function method mkTwoNode(left: Node, pivot: int, right: Node) : Node {
+	TwoNode(left, pivot, right, IntervalUnion(SummaryInterval(left), SummaryInterval(right)))
+}
+						
+function method mkThreeNode(left: Node, pivota: int, middle: Node, pivotb: int, right: Node) : Node {
+	ThreeNode(left, pivota, middle, pivotb, right,
+		IntervalUnion3(SummaryInterval(left), SummaryInterval(middle), SummaryInterval(right)))
+}
+
+function SubtreeContents(tree: Node) : set<Interval>
+	ensures SubtreeContents(tree) != {};
+{
+	if tree.Leaf?
+		then {tree.value}
+	else if tree.TwoNode?
+    then SubtreeContents(tree.left) + SubtreeContents(tree.right)
+	else 
+		SubtreeContents(tree.left) + SubtreeContents(tree.middle) + SubtreeContents(tree.right)
+}
+
+predicate OrderedTree(tree: Node)
+{
+    if tree.Leaf?
+			then true
+		else if tree.TwoNode?
+      then
+			(forall intrvl: Interval :: intrvl in SubtreeContents(tree) ==> IsSubInterval(intrvl, tree.interval)) &&
+			(forall intrvl: Interval :: intrvl in SubtreeContents(tree.left) ==> intrvl.low.point <= tree.pivot) &&
+			(forall intrvl: Interval :: intrvl in SubtreeContents(tree.right) ==> tree.pivot <= intrvl.low.point) &&
+			OrderedTree(tree.left) &&
+			OrderedTree(tree.right)
+		else
+			tree.pivota <= tree.pivotb &&
+			(forall intrvl: Interval :: intrvl in SubtreeContents(tree) ==> IsSubInterval(intrvl, tree.interval)) &&
+			(forall intrvl: Interval :: intrvl in SubtreeContents(tree.left) ==> intrvl.low.point <= tree.pivota) &&
+			(forall intrvl: Interval :: intrvl in SubtreeContents(tree.middle) ==> tree.pivota <= intrvl.low.point &&
+			                                                               intrvl.low.point <= tree.pivotb) &&
+			(forall intrvl: Interval :: intrvl in SubtreeContents(tree.right) ==> tree.pivotb <= intrvl.low.point) &&
+			OrderedTree(tree.left) &&
+			OrderedTree(tree.middle) &&
+			OrderedTree(tree.right)
+}
+
+function method StabbingQuery(tree: Node, value: int) : set<Interval>
+  requires OrderedTree(tree);
+	ensures StabbingQuery(tree, value) ==
+	 	set ival : Interval | ival in SubtreeContents(tree) && IntervalContains(ival, value)
+{
+	match tree {
+		case Leaf(ival) =>
+			if IntervalContains(ival, value) then {ival} else {}
+		case TwoNode(left, pivot, right, sumintrvl) =>
+			if !IntervalContains(sumintrvl, value) then
+			{}
+			else
+				StabbingQuery(left, value) + StabbingQuery(right, value)
+		case ThreeNode(left, pivota, middle, pivotb, right, sumintrvl) =>
+			if !IntervalContains(sumintrvl, value) then
+			{}
+			else
+				StabbingQuery(left, value) + StabbingQuery(middle, value) + StabbingQuery(right, value)
+	}
+}
+
+function minHeight(tree: Node) : int
+{
+	if tree.Leaf?
+		then 0
+	else if tree.TwoNode?
+		then 1 + min(minHeight(tree.left), minHeight(tree.right))
+	else 
+		1 + min(minHeight(tree.left), min(minHeight(tree.middle), minHeight(tree.right)))
+}
+
+function maxHeight(tree: Node) : int
+{
+	if tree.Leaf?
+		then 0
+	else if tree.TwoNode?
+		then 1 + max(maxHeight(tree.left), maxHeight(tree.right))
+	else
+		1 + max(maxHeight(tree.left), max(maxHeight(tree.middle), maxHeight(tree.right)))
+}
+
+predicate Balanced(tree: Node)
+{
+	minHeight(tree) == maxHeight(tree) &&
+		(tree.TwoNode? ==> Balanced(tree.left) && Balanced(tree.right)) &&
+		(tree.ThreeNode? ==> Balanced(tree.left) && Balanced(tree.middle) && Balanced(tree.right))
+}
+
+predicate ITTSubtree(tree: Node) {
+
+	if tree.Leaf? then
+		OrderedTree(tree) &&
+		Balanced(tree) &&
+		SubtreeContents(tree) != {}
+	else if tree.TwoNode? then
+		OrderedTree(tree) &&
+		Balanced(tree) &&
+		SubtreeContents(tree) != {} &&
+		ITTSubtree(tree.left) &&
+		ITTSubtree(tree.right)
+	else
+		OrderedTree(tree) &&
+		Balanced(tree) &&
+		SubtreeContents(tree) != {} &&
+		ITTSubtree(tree.left) &&
+		ITTSubtree(tree.middle) &&
+		ITTSubtree(tree.right)
+}
+
+function method Height(tree: Node) : int
+	requires Balanced(tree);
+	ensures Height(tree) == minHeight(tree);
+	ensures Height(tree) == maxHeight(tree);
+{
+	if tree.Leaf? then 0 else 1 + Height(tree.left)
+}
+
+datatype InsertionResult = InsertionResult(tree: Node, split: bool)
+	
+method InternalInsert(tree: Node, intrvl: Interval) returns (result: InsertionResult)
+	requires ITTSubtree(tree);
+	ensures ITTSubtree(result.tree);
+	ensures SubtreeContents(result.tree) == SubtreeContents(tree) + {intrvl};
+	ensures result.split ==> Height(result.tree) == Height(tree) + 1;
+	ensures result.split ==> result.tree.TwoNode?;
+	ensures !result.split ==> Height(result.tree) == Height(tree);
+{
+	if tree.Leaf? {
+		if tree.value == intrvl {
+			result := InsertionResult(tree, false);
+		} else if tree.value.low.point < intrvl.low.point {
+			var newright := Leaf(intrvl);
+			var newtree := mkTwoNode(tree, intrvl.low.point, newright);
+			assert(Height(newright) == Height(tree));
+			assert(Height(newtree) == Height(tree) + 1);
+			result := InsertionResult(newtree, true);
+		} else {
+			var newleft := Leaf(intrvl);
+			var newtree := mkTwoNode(newleft, tree.value.low.point, tree);
+			assert(Height(newleft) == Height(tree));
+			assert(Height(newtree) == Height(tree) + 1);
+			result := InsertionResult(newtree, true);
+		}
+	} else if tree.TwoNode? {
+		if intrvl.low.point < tree.pivot {
+			var subresult := InternalInsert(tree.left, intrvl);
+			if !subresult.split {
+				result := InsertionResult(mkTwoNode(subresult.tree, tree.pivot, tree.right), false);
+			} else {
+				result := InsertionResult(mkThreeNode(subresult.tree.left, subresult.tree.pivot,
+					                                   subresult.tree.right, tree.pivot,
+																					   tree.right),
+																 false);
+			}
+		} else {
+			var subresult := InternalInsert(tree.right, intrvl);
+			if !subresult.split {
+				result := InsertionResult(mkTwoNode(tree.left, tree.pivot, subresult.tree), false);
+			} else {
+				result := InsertionResult(mkThreeNode(tree.left, tree.pivot,
+			                		                   subresult.tree.left, subresult.tree.pivot,
+																		 				 subresult.tree.right), false);
+			}
+		}
+	} else if tree.ThreeNode? {
+		if intrvl.low.point < tree.pivota {
+			var subresult := InternalInsert(tree.left, intrvl);
+			if !subresult.split {
+				result := InsertionResult(mkThreeNode(subresult.tree, tree.pivota,
+					                                   tree.middle, tree.pivotb,
+																						 tree.right), false);
+			} else {
+				var newright := mkTwoNode(tree.middle, tree.pivotb, tree.right);
+				assert(Height(newright) == Height(tree));
+				var newtree := mkTwoNode(subresult.tree, tree.pivota, newright);
+				assert(Height(newtree) == Height(tree) + 1);
+				result := InsertionResult(newtree, true);
+			}
+		} else if intrvl.low.point < tree.pivotb {
+			var subresult := InternalInsert(tree.middle, intrvl);
+			if !subresult.split {
+				result := InsertionResult(mkThreeNode(tree.left, tree.pivota,
+					                                   subresult.tree, tree.pivotb,
+																						 tree.right), false);
+			} else {
+				var newleft := mkTwoNode(tree.left, tree.pivota, subresult.tree.left);
+				var newright := mkTwoNode(subresult.tree.right, tree.pivotb, tree.right);
+				var newtree := mkTwoNode(newleft, subresult.tree.pivot, newright);
+				assert(Height(newleft) == Height(tree));
+				assert(Height(newright) == Height(tree));
+				assert(Height(newtree) == Height(tree) + 1);
+				result := InsertionResult(newtree, true);
+				}
+		} else {
+			var subresult := InternalInsert(tree.right, intrvl);
+			if !subresult.split {
+				result := InsertionResult(mkThreeNode(tree.left, tree.pivota,
+					                                   tree.middle, tree.pivotb,
+																						 subresult.tree), false);
+			} else {
+				var newleft := mkTwoNode(tree.left, tree.pivota, tree.middle);
+				var newtree := mkTwoNode(newleft, tree.pivotb, subresult.tree);
+				assert(Height(newleft) == Height(tree));
+				assert(Height(newtree) == Height(tree) + 1);
+				result := InsertionResult(newtree, true);
+			}
+		}
+	} 
+}
+
+// datatype Tree = EmptyTree | NonEmptyTree(root: Node)
+
+// predicate TTTree(tree: Tree) {
+// 	tree.EmptyTree? || TTSubtree(tree.root)
+// }
+
+// function Contents(tree: Tree) : set<int>
+// {
+// 	if tree.EmptyTree?
+// 		then {}
+// 	else
+// 		SubtreeContents(tree.root)
+// }
+
+// method Contains(tree: Tree, value: int) returns (present: bool)
+// 	requires(TTTree(tree));
+// 	ensures(present == (value in Contents(tree)));
+// {
+// 	if tree.EmptyTree? {
+// 		present := false;
+// 	} else { 
+// 		present := NodeContains(tree.root, value);
+// 	}
+// }
+
+// method Insert(tree: Tree, value: int) returns (newtree: Tree)
+// 	requires(TTTree(tree));
+// 	ensures(TTTree(newtree));
+// 	ensures(Contents(newtree) == Contents(tree) + {value});
+// 	ensures(newtree.NonEmptyTree?);
+// {
+// 	if tree.EmptyTree? {
+// 		newtree := NonEmptyTree(Leaf(value));
+// 	} else {
+// 		var result := InternalInsert(tree.root, value);
+// 		newtree := NonEmptyTree(result.tree);
+// 	}
+// }
